\section{Q5}
\label{s:Q5}
$$X \geq x \implies e^{sX} \geq e^{sx} (s >0)$$
$$\implies \mathbb{P}(X \geq x) = \mathbb{P}(e^{sX} \geq e^{sx}) \leq e^{-sx}\mathbb{E}[e^{sX}]$$
Defining the right-hand side as follows:
$$\underset{s}{\text{min}} f(s) \Let e^{-sx}\mathbb{E}[e^{sX}] = e^{-sx}\int_{-\infty}^{\infty}e^{sy}\frac{1}{\sqrt{2\pi}}e^{\frac{-y^2}{2}}dy$$

Computing the definite integral yields:
$$\underset{s}{\text{min}} f(s) \Let e^{-sx}\mathbb{E}[e^{sX}] = e^{-sx + \frac{s^2}{2}}$$

The minimum occurs at $s=x \implies \mathbb{P}(X \geq x) = \mathbb{P}(e^{sX} \geq e^{sx}) \leq e^{\frac{-x^2}{2}}.$

